src/FairSim.v
@@ -14,16 +14,16 @@ Set Implicit Arguments.
 
 Section SIM.
 
-  Variable Ident: Type.
+  Context {Ident: ID}.
 
-  Definition fmap := Ident -> Flag.t.
+  Definition fmap := Ident.(id) -> Flag.t.
   Definition fmap_emp : fmap := fun _ => Flag.emp.
 
   Inductive _sim
             (sim: forall R0 R1 (RR: R0 -> R1 -> Prop),
-                bool -> fmap  -> bool -> fmap -> Ident -> (itree (eventE Ident) R0) -> (itree (eventE Ident) R1) -> Prop)
-            {R0 R1} (RR: R0 -> R1 -> Prop) (p_src: bool) (m_src: fmap) (p_tgt: bool) (m_tgt: fmap) (idx: Ident) :
-    (itree (eventE _) R0) -> (itree (eventE _) R1) -> Prop :=
+                bool -> fmap  -> bool -> fmap -> Ident.(id) -> (itree eventE R0) -> (itree eventE R1) -> Prop)
+            {R0 R1} (RR: R0 -> R1 -> Prop) (p_src: bool) (m_src: fmap) (p_tgt: bool) (m_tgt: fmap) (idx: Ident.(id)) :
+    (itree eventE R0) -> (itree eventE R1) -> Prop :=
   | sim_ret
       r_src r_tgt
       (SIM: RR r_src r_tgt)
@@ -44,42 +44,23 @@ Section SIM.
       X ktr_src0 itr_tgt0
       (SIM: exists x, _sim sim RR true m_src p_tgt m_tgt idx (ktr_src0 x) itr_tgt0)
     :
-    _sim sim RR p_src m_src p_tgt m_tgt idx (trigger (Choose _ X) >>= ktr_src0) itr_tgt0
+    _sim sim RR p_src m_src p_tgt m_tgt idx (trigger (Choose X) >>= ktr_src0) itr_tgt0
   | sim_chooseR
       X itr_src0 ktr_tgt0
       (SIM: forall x, _sim sim RR p_src m_src true m_tgt idx itr_src0 (ktr_tgt0 x))
     :
-    _sim sim RR p_src m_src p_tgt m_tgt idx itr_src0 (trigger (Choose _ X) >>= ktr_tgt0)
+    _sim sim RR p_src m_src p_tgt m_tgt idx itr_src0 (trigger (Choose X) >>= ktr_tgt0)
 
-  | sim_failL
-      id m_src0 ktr_src0 itr_tgt0
-      (SRC: forall j, Flag.le (m_src0 j) (m_src j))
-      (FAIL: (Flag.le (m_src id) Flag.emp) -> (Flag.le (m_src0 id) Flag.fail))
+  | sim_fairL
+      m_src0 ktr_src0 itr_tgt0
       (SIM: _sim sim RR true m_src0 p_tgt m_tgt idx (ktr_src0 tt) itr_tgt0)
     :
-    _sim sim RR p_src m_src p_tgt m_tgt idx (trigger (Fail id) >>= ktr_src0) itr_tgt0
-  | sim_failR
-      id m_tgt0 itr_src0 ktr_tgt0
-      (TGT: forall j, Flag.le (m_tgt0 j) (m_tgt j))
-      (FAIL: (Flag.le (m_tgt id) Flag.emp) -> (Flag.le (m_tgt0 id) Flag.fail))
+    _sim sim RR p_src m_src p_tgt m_tgt idx (trigger (Fair m_src0) >>= ktr_src0) itr_tgt0
+  | sim_fairR
+      m_tgt0 itr_src0 ktr_tgt0
       (SIM: _sim sim RR p_src m_src true m_tgt0 idx itr_src0 (ktr_tgt0 tt))
     :
-    _sim sim RR p_src m_src p_tgt m_tgt idx itr_src0 (trigger (Fail id) >>= ktr_tgt0)
-
-  | sim_successL
-      id m_src0 ktr_src0 itr_tgt0
-      (SRC: forall j (NEQ: id <> j), Flag.le (m_src0 j) (m_src j))
-      (SUCCESS: Flag.le Flag.success (m_src0 id))
-      (SIM: _sim sim RR true m_src0 p_tgt m_tgt idx (ktr_src0 tt) itr_tgt0)
-    :
-    _sim sim RR p_src m_src p_tgt m_tgt idx (trigger (Success id) >>= ktr_src0) itr_tgt0
-  | sim_successR
-      id m_tgt0 itr_src0 ktr_tgt0
-      (TGT: forall j (NEQ: id <> j), Flag.le (m_tgt0 j) (m_tgt j))
-      (SUCCESS: Flag.le Flag.success (m_tgt0 id))
-      (SIM: _sim sim RR p_src m_src true m_tgt0 idx itr_src0 (ktr_tgt0 tt))
-    :
-    _sim sim RR p_src m_src p_tgt m_tgt idx itr_src0 (trigger (Success id) >>= ktr_tgt0)
+    _sim sim RR p_src m_src p_tgt m_tgt idx itr_src0 (trigger (Fair m_tgt0) >>= ktr_tgt0)
 
   | sim_progress_strong
       itr_src0 itr_tgt0 idx0
@@ -101,9 +82,9 @@ Section SIM.
     _sim sim RR p_src m_src p_tgt m_tgt idx itr_src0 itr_tgt0
   .
 
-  Lemma _sim_ind2 (r: forall R0 R1 (RR: R0 -> R1 -> Prop), bool -> fmap  -> bool -> fmap -> Ident -> (itree (eventE Ident) R0) -> (itree (eventE Ident) R1) -> Prop)
+  Lemma _sim_ind2 (r: forall R0 R1 (RR: R0 -> R1 -> Prop), bool -> fmap  -> bool -> fmap -> Ident.(id) -> (itree eventE R0) -> (itree eventE R1) -> Prop)
         R0 R1 (RR: R0 -> R1 -> Prop)
-        (P: bool -> fmap  -> bool -> fmap -> Ident -> (itree (eventE Ident) R0) -> (itree (eventE Ident) R1) -> Prop)
+        (P: bool -> fmap  -> bool -> fmap -> Ident.(id) -> (itree eventE R0) -> (itree eventE R1) -> Prop)
         (RET: forall
             p_src m_src p_tgt m_tgt idx
             r_src r_tgt
@@ -124,44 +105,24 @@ Section SIM.
             p_src m_src p_tgt m_tgt idx X ktr_src0 itr_tgt0
             (SIM: exists x, <<SIM: _sim r RR true m_src p_tgt m_tgt idx (ktr_src0 x) itr_tgt0>> /\
                                 <<IH: P true m_src p_tgt m_tgt idx (ktr_src0 x) itr_tgt0>>),
-            P p_src m_src p_tgt m_tgt idx (ITree.bind (trigger (Choose _ X)) ktr_src0) itr_tgt0)
+            P p_src m_src p_tgt m_tgt idx (ITree.bind (trigger (Choose X)) ktr_src0) itr_tgt0)
         (CHOOSER: forall
             p_src m_src p_tgt m_tgt idx X itr_src0 ktr_tgt0
             (SIM: forall x, <<SIM: _sim r RR p_src m_src true m_tgt idx itr_src0 (ktr_tgt0 x)>> /\
                                 <<IH: P p_src m_src true m_tgt idx itr_src0 (ktr_tgt0 x)>>),
-            P p_src m_src p_tgt m_tgt idx itr_src0 (ITree.bind (trigger (Choose _ X)) ktr_tgt0))
-        (FAILL: forall
+            P p_src m_src p_tgt m_tgt idx itr_src0 (ITree.bind (trigger (Choose X)) ktr_tgt0))
+        (FAIRL: forall
             p_src m_src p_tgt m_tgt idx ktr_src0 itr_tgt0
-            id m_src0
-            (SRC: forall j, Flag.le (m_src0 j) (m_src j))
-            (FAIL: (Flag.le (m_src id) Flag.emp) -> (Flag.le (m_src0 id) Flag.fail))
+            m_src0
             (SIM: _sim r RR true m_src0 p_tgt m_tgt idx (ktr_src0 tt) itr_tgt0)
             (IH: P true m_src0 p_tgt m_tgt idx (ktr_src0 tt) itr_tgt0),
-            P p_src m_src p_tgt m_tgt idx (ITree.bind (trigger (Fail id)) ktr_src0) itr_tgt0)
-        (FAILR: forall
+            P p_src m_src p_tgt m_tgt idx (ITree.bind (trigger (Fair m_src0)) ktr_src0) itr_tgt0)
+        (FAIRR: forall
             p_src m_src p_tgt m_tgt idx itr_src0 ktr_tgt0
-            id m_tgt0
-            (TGT: forall j, Flag.le (m_tgt0 j) (m_tgt j))
-            (FAIL: (Flag.le (m_tgt id) Flag.emp) -> (Flag.le (m_tgt0 id) Flag.fail))
+            m_tgt0
             (SIM: _sim r RR p_src m_src true m_tgt0 idx itr_src0 (ktr_tgt0 tt))
             (IH: P p_src m_src true m_tgt0 idx itr_src0 (ktr_tgt0 tt)),
-            P p_src m_src p_tgt m_tgt idx itr_src0 (ITree.bind (trigger (Fail id)) ktr_tgt0))
-        (SUCCESSL: forall
-            p_src m_src p_tgt m_tgt idx ktr_src0 itr_tgt0
-            id m_src0
-            (SRC: forall j (NEQ: id <> j), Flag.le (m_src0 j) (m_src j))
-            (SUCCESS: Flag.le Flag.success (m_src0 id))
-            (SIM: _sim r RR true m_src0 p_tgt m_tgt idx (ktr_src0 tt) itr_tgt0)
-            (IH: P true m_src0 p_tgt m_tgt idx (ktr_src0 tt) itr_tgt0),
-            P p_src m_src p_tgt m_tgt idx (ITree.bind (trigger (Success id)) ktr_src0) itr_tgt0)
-        (SUCCESSR: forall
-            p_src m_src p_tgt m_tgt idx itr_src0 ktr_tgt0
-            id m_tgt0
-            (TGT: forall j (NEQ: id <> j), Flag.le (m_tgt0 j) (m_tgt j))
-            (SUCCESS: Flag.le Flag.success (m_tgt0 id))
-            (SIM: _sim r RR p_src m_src true m_tgt0 idx itr_src0 (ktr_tgt0 tt))
-            (IH: P p_src m_src true m_tgt0 idx itr_src0 (ktr_tgt0 tt)),
-            P p_src m_src p_tgt m_tgt idx itr_src0 (ITree.bind (trigger (Success id)) ktr_tgt0))
+            P p_src m_src p_tgt m_tgt idx itr_src0 (ITree.bind (trigger (Fair m_tgt0)) ktr_tgt0))
         (PROGRESSS: forall
             p_src m_src p_tgt m_tgt idx itr_src0 itr_tgt0
             idx0
@@ -190,15 +151,13 @@ Section SIM.
     { eapply TAUR; eauto. }
     { eapply CHOOSEL; eauto. des. esplits; eauto. }
     { eapply CHOOSER; eauto. }
-    { eapply FAILL; eauto. }
-    { eapply FAILR; eauto. }
-    { eapply SUCCESSL; eauto. }
-    { eapply SUCCESSR; eauto. }
+    { eapply FAIRL; eauto. }
+    { eapply FAIRR; eauto. }
     { eapply PROGRESSS; eauto. }
     { eapply PROGRESSW; eauto. }
   Qed.
 
-  Definition sim: forall R0 R1 (RR: R0 -> R1 -> Prop), bool -> fmap  -> bool -> fmap -> Ident -> (itree (eventE _) R0) -> (itree (eventE _) R1) -> Prop := paco10 _sim bot10.
+  Definition sim: forall R0 R1 (RR: R0 -> R1 -> Prop), bool -> fmap  -> bool -> fmap -> Ident.(id) -> (itree eventE R0) -> (itree eventE R1) -> Prop := paco10 _sim bot10.
 
   Lemma sim_mon: monotone10 _sim.
   Proof.
@@ -212,8 +171,6 @@ Section SIM.
     { econs 7; eauto. }
     { econs 8; eauto. }
     { econs 9; eauto. }
-    { econs 10; eauto. }
-    { econs 11; eauto. }
   Qed.
 
   Hint Resolve sim_mon: paco.
@@ -221,178 +178,178 @@ Section SIM.
 
 
 
-  Definition imap := Ident -> nat.
+  (* Definition imap := Ident -> nat. *)
 
-  Inductive _isim
-            (isim: forall R0 R1 (RR: R0 -> R1 -> Prop),
-                bool -> imap  -> bool -> imap -> (itree (eventE Ident) R0) -> (itree (eventE Ident) R1) -> Prop)
-            {R0 R1} (RR: R0 -> R1 -> Prop) (p_src: bool) (m_src: imap) (p_tgt: bool) (m_tgt: imap):
-    (itree (eventE Ident) R0) -> (itree (eventE Ident) R1) -> Prop :=
-  | isim_ret
-      r_src r_tgt
-      (SIM: RR r_src r_tgt)
-    :
-    _isim isim RR p_src m_src p_tgt m_tgt (Ret r_src) (Ret r_tgt)
-  | isim_tauL
-      itr_src0 itr_tgt0
-      (SIM: @_isim isim _ _ RR true m_src p_tgt m_tgt itr_src0 itr_tgt0)
-    :
-    _isim isim RR p_src m_src p_tgt m_tgt (Tau itr_src0) itr_tgt0
-  | isim_tauR
-      itr_src0 itr_tgt0
-      (SIM: @_isim isim _ _ RR p_src m_src true m_tgt itr_src0 itr_tgt0)
-    :
-    _isim isim RR p_src m_src p_tgt m_tgt itr_src0 (Tau itr_tgt0)
-  | isim_chooseL
-      X ktr_src0 itr_tgt0
-      (SIM: exists x, _isim isim RR true m_src p_tgt m_tgt (ktr_src0 x) itr_tgt0)
-    :
-    _isim isim RR p_src m_src p_tgt m_tgt (trigger (Choose _ X) >>= ktr_src0) itr_tgt0
-  | isim_chooseR
-      X itr_src0 ktr_tgt0
-      (SIM: forall x, _isim isim RR p_src m_src true m_tgt itr_src0 (ktr_tgt0 x))
-    :
-    _isim isim RR p_src m_src p_tgt m_tgt itr_src0 (trigger (Choose _ X) >>= ktr_tgt0)
+  (* Inductive _isim *)
+  (*           (isim: forall R0 R1 (RR: R0 -> R1 -> Prop), *)
+  (*               bool -> imap  -> bool -> imap -> (itree (eventE Ident) R0) -> (itree (eventE Ident) R1) -> Prop) *)
+  (*           {R0 R1} (RR: R0 -> R1 -> Prop) (p_src: bool) (m_src: imap) (p_tgt: bool) (m_tgt: imap): *)
+  (*   (itree (eventE Ident) R0) -> (itree (eventE Ident) R1) -> Prop := *)
+  (* | isim_ret *)
+  (*     r_src r_tgt *)
+  (*     (SIM: RR r_src r_tgt) *)
+  (*   : *)
+  (*   _isim isim RR p_src m_src p_tgt m_tgt (Ret r_src) (Ret r_tgt) *)
+  (* | isim_tauL *)
+  (*     itr_src0 itr_tgt0 *)
+  (*     (SIM: @_isim isim _ _ RR true m_src p_tgt m_tgt itr_src0 itr_tgt0) *)
+  (*   : *)
+  (*   _isim isim RR p_src m_src p_tgt m_tgt (Tau itr_src0) itr_tgt0 *)
+  (* | isim_tauR *)
+  (*     itr_src0 itr_tgt0 *)
+  (*     (SIM: @_isim isim _ _ RR p_src m_src true m_tgt itr_src0 itr_tgt0) *)
+  (*   : *)
+  (*   _isim isim RR p_src m_src p_tgt m_tgt itr_src0 (Tau itr_tgt0) *)
+  (* | isim_chooseL *)
+  (*     X ktr_src0 itr_tgt0 *)
+  (*     (SIM: exists x, _isim isim RR true m_src p_tgt m_tgt (ktr_src0 x) itr_tgt0) *)
+  (*   : *)
+  (*   _isim isim RR p_src m_src p_tgt m_tgt (trigger (Choose _ X) >>= ktr_src0) itr_tgt0 *)
+  (* | isim_chooseR *)
+  (*     X itr_src0 ktr_tgt0 *)
+  (*     (SIM: forall x, _isim isim RR p_src m_src true m_tgt itr_src0 (ktr_tgt0 x)) *)
+  (*   : *)
+  (*   _isim isim RR p_src m_src p_tgt m_tgt itr_src0 (trigger (Choose _ X) >>= ktr_tgt0) *)
 
-  | isim_failL
-      id m_src0 ktr_src0 itr_tgt0
-      (SRC: forall j, le (m_src0 j) (m_src j))
-      (FAIL: lt (m_src0 id) (m_src id))
-      (SIM: _isim isim RR true m_src0 p_tgt m_tgt (ktr_src0 tt) itr_tgt0)
-    :
-    _isim isim RR p_src m_src p_tgt m_tgt (trigger (Fail id) >>= ktr_src0) itr_tgt0
-  | isim_failR
-      id itr_src0 ktr_tgt0
-      (SIM: forall m_tgt0 (TGT: forall j, le (m_tgt0 j) (m_tgt j)) (FAIL: lt (m_tgt0 id) (m_tgt id)),
-          _isim isim RR p_src m_src true m_tgt0 itr_src0 (ktr_tgt0 tt))
-    :
-    _isim isim RR p_src m_src p_tgt m_tgt itr_src0 (trigger (Fail id) >>= ktr_tgt0)
+  (* | isim_failL *)
+  (*     id m_src0 ktr_src0 itr_tgt0 *)
+  (*     (SRC: forall j, le (m_src0 j) (m_src j)) *)
+  (*     (FAIL: lt (m_src0 id) (m_src id)) *)
+  (*     (SIM: _isim isim RR true m_src0 p_tgt m_tgt (ktr_src0 tt) itr_tgt0) *)
+  (*   : *)
+  (*   _isim isim RR p_src m_src p_tgt m_tgt (trigger (Fail id) >>= ktr_src0) itr_tgt0 *)
+  (* | isim_failR *)
+  (*     id itr_src0 ktr_tgt0 *)
+  (*     (SIM: forall m_tgt0 (TGT: forall j, le (m_tgt0 j) (m_tgt j)) (FAIL: lt (m_tgt0 id) (m_tgt id)), *)
+  (*         _isim isim RR p_src m_src true m_tgt0 itr_src0 (ktr_tgt0 tt)) *)
+  (*   : *)
+  (*   _isim isim RR p_src m_src p_tgt m_tgt itr_src0 (trigger (Fail id) >>= ktr_tgt0) *)
 
-  | isim_successL
-      id m_src0 ktr_src0 itr_tgt0
-      (SRC: forall j (NEQ: id <> j), le (m_src0 j) (m_src j))
-      (SIM: _isim isim RR true m_src0 p_tgt m_tgt (ktr_src0 tt) itr_tgt0)
-    :
-    _isim isim RR p_src m_src p_tgt m_tgt (trigger (Success id) >>= ktr_src0) itr_tgt0
-  | isim_successR
-      id itr_src0 ktr_tgt0
-      (SIM: forall m_tgt0 (TGT: forall j (NEQ: id <> j), le (m_tgt0 j) (m_tgt j)),
-          _isim isim RR p_src m_src true m_tgt0 itr_src0 (ktr_tgt0 tt))
-    :
-    _isim isim RR p_src m_src p_tgt m_tgt itr_src0 (trigger (Success id) >>= ktr_tgt0)
+  (* | isim_successL *)
+  (*     id m_src0 ktr_src0 itr_tgt0 *)
+  (*     (SRC: forall j (NEQ: id <> j), le (m_src0 j) (m_src j)) *)
+  (*     (SIM: _isim isim RR true m_src0 p_tgt m_tgt (ktr_src0 tt) itr_tgt0) *)
+  (*   : *)
+  (*   _isim isim RR p_src m_src p_tgt m_tgt (trigger (Success id) >>= ktr_src0) itr_tgt0 *)
+  (* | isim_successR *)
+  (*     id itr_src0 ktr_tgt0 *)
+  (*     (SIM: forall m_tgt0 (TGT: forall j (NEQ: id <> j), le (m_tgt0 j) (m_tgt j)), *)
+  (*         _isim isim RR p_src m_src true m_tgt0 itr_src0 (ktr_tgt0 tt)) *)
+  (*   : *)
+  (*   _isim isim RR p_src m_src p_tgt m_tgt itr_src0 (trigger (Success id) >>= ktr_tgt0) *)
 
-  | isim_progress_strong
-      itr_src0 itr_tgt0
-      (PSRC: p_src = true)
-      (PTGT: p_tgt = true)
-      (IMAP: forall j, (<<SRC: forall n, le (m_src j) n>>) -> (<<TGT: forall n, le (m_tgt j) n>>))
-      (SIM: exists m_src0 m_tgt0, isim _ _ RR false m_src0 false m_tgt0 itr_src0 itr_tgt0)
-    :
-    _isim isim RR p_src m_src p_tgt m_tgt itr_src0 itr_tgt0
-  .
+  (* | isim_progress_strong *)
+  (*     itr_src0 itr_tgt0 *)
+  (*     (PSRC: p_src = true) *)
+  (*     (PTGT: p_tgt = true) *)
+  (*     (IMAP: forall j, (<<SRC: forall n, le (m_src j) n>>) -> (<<TGT: forall n, le (m_tgt j) n>>)) *)
+  (*     (SIM: exists m_src0 m_tgt0, isim _ _ RR false m_src0 false m_tgt0 itr_src0 itr_tgt0) *)
+  (*   : *)
+  (*   _isim isim RR p_src m_src p_tgt m_tgt itr_src0 itr_tgt0 *)
+  (* . *)
 
-  Lemma _isim_ind2 (r: forall R0 R1 (RR: R0 -> R1 -> Prop), bool -> imap  -> bool -> imap -> (itree (eventE Ident) R0) -> (itree (eventE Ident) R1) -> Prop)
-        R0 R1 (RR: R0 -> R1 -> Prop)
-        (P: bool -> imap  -> bool -> imap -> (itree (eventE Ident) R0) -> (itree (eventE Ident) R1) -> Prop)
-        (RET: forall
-            p_src m_src p_tgt m_tgt
-            r_src r_tgt
-            (SIM: RR r_src r_tgt),
-            P p_src m_src p_tgt m_tgt (Ret r_src) (Ret r_tgt))
-        (TAUL: forall 
-            p_src m_src p_tgt m_tgt itr_src0 itr_tgt0
-            (SIM: _isim r RR true m_src p_tgt m_tgt itr_src0 itr_tgt0)
-            (IH: P true m_src p_tgt m_tgt itr_src0 itr_tgt0),
-            P p_src m_src p_tgt m_tgt (Tau itr_src0) itr_tgt0)
-        (TAUR: forall 
-            p_src m_src p_tgt m_tgt itr_src0 itr_tgt0
-            (SIM: _isim r RR p_src m_src true m_tgt itr_src0 itr_tgt0)
-            (IH: P p_src m_src true m_tgt itr_src0 itr_tgt0),
-            P p_src m_src p_tgt m_tgt itr_src0 (Tau itr_tgt0))
-        (CHOOSEL: forall
-            p_src m_src p_tgt m_tgt X ktr_src0 itr_tgt0
-            (SIM: exists x, <<SIM: _isim r RR true m_src p_tgt m_tgt (ktr_src0 x) itr_tgt0>> /\
-                                <<IH: P true m_src p_tgt m_tgt (ktr_src0 x) itr_tgt0>>),
-            P p_src m_src p_tgt m_tgt (ITree.bind (trigger (Choose _ X)) ktr_src0) itr_tgt0)
-        (CHOOSER: forall
-            p_src m_src p_tgt m_tgt X itr_src0 ktr_tgt0
-            (SIM: forall x, <<SIM: _isim r RR p_src m_src true m_tgt itr_src0 (ktr_tgt0 x)>> /\
-                                <<IH: P p_src m_src true m_tgt itr_src0 (ktr_tgt0 x)>>),
-            P p_src m_src p_tgt m_tgt itr_src0 (ITree.bind (trigger (Choose _ X)) ktr_tgt0))
-        (FAILL: forall
-            p_src m_src p_tgt m_tgt ktr_src0 itr_tgt0
-            id m_src0
-            (SRC: forall j, le (m_src0 j) (m_src j))
-            (FAIL: lt (m_src0 id) (m_src id))
-            (SIM: _isim r RR true m_src0 p_tgt m_tgt (ktr_src0 tt) itr_tgt0)
-            (IH: P true m_src0 p_tgt m_tgt (ktr_src0 tt) itr_tgt0),
-            P p_src m_src p_tgt m_tgt (ITree.bind (trigger (Fail id)) ktr_src0) itr_tgt0)
-        (FAILR: forall
-            p_src m_src p_tgt m_tgt itr_src0 ktr_tgt0
-            id
-            (SIM: forall m_tgt0 (TGT: forall j, le (m_tgt0 j) (m_tgt j)) (FAIL: lt (m_tgt0 id) (m_tgt id)),
-                (<<SIM: _isim r RR p_src m_src true m_tgt0 itr_src0 (ktr_tgt0 tt)>> /\
-                          (<<IH: P p_src m_src true m_tgt0 itr_src0 (ktr_tgt0 tt)>>))),
-            P p_src m_src p_tgt m_tgt itr_src0 (ITree.bind (trigger (Fail id)) ktr_tgt0))
+  (* Lemma _isim_ind2 (r: forall R0 R1 (RR: R0 -> R1 -> Prop), bool -> imap  -> bool -> imap -> (itree (eventE Ident) R0) -> (itree (eventE Ident) R1) -> Prop) *)
+  (*       R0 R1 (RR: R0 -> R1 -> Prop) *)
+  (*       (P: bool -> imap  -> bool -> imap -> (itree (eventE Ident) R0) -> (itree (eventE Ident) R1) -> Prop) *)
+  (*       (RET: forall *)
+  (*           p_src m_src p_tgt m_tgt *)
+  (*           r_src r_tgt *)
+  (*           (SIM: RR r_src r_tgt), *)
+  (*           P p_src m_src p_tgt m_tgt (Ret r_src) (Ret r_tgt)) *)
+  (*       (TAUL: forall  *)
+  (*           p_src m_src p_tgt m_tgt itr_src0 itr_tgt0 *)
+  (*           (SIM: _isim r RR true m_src p_tgt m_tgt itr_src0 itr_tgt0) *)
+  (*           (IH: P true m_src p_tgt m_tgt itr_src0 itr_tgt0), *)
+  (*           P p_src m_src p_tgt m_tgt (Tau itr_src0) itr_tgt0) *)
+  (*       (TAUR: forall  *)
+  (*           p_src m_src p_tgt m_tgt itr_src0 itr_tgt0 *)
+  (*           (SIM: _isim r RR p_src m_src true m_tgt itr_src0 itr_tgt0) *)
+  (*           (IH: P p_src m_src true m_tgt itr_src0 itr_tgt0), *)
+  (*           P p_src m_src p_tgt m_tgt itr_src0 (Tau itr_tgt0)) *)
+  (*       (CHOOSEL: forall *)
+  (*           p_src m_src p_tgt m_tgt X ktr_src0 itr_tgt0 *)
+  (*           (SIM: exists x, <<SIM: _isim r RR true m_src p_tgt m_tgt (ktr_src0 x) itr_tgt0>> /\ *)
+  (*                               <<IH: P true m_src p_tgt m_tgt (ktr_src0 x) itr_tgt0>>), *)
+  (*           P p_src m_src p_tgt m_tgt (ITree.bind (trigger (Choose _ X)) ktr_src0) itr_tgt0) *)
+  (*       (CHOOSER: forall *)
+  (*           p_src m_src p_tgt m_tgt X itr_src0 ktr_tgt0 *)
+  (*           (SIM: forall x, <<SIM: _isim r RR p_src m_src true m_tgt itr_src0 (ktr_tgt0 x)>> /\ *)
+  (*                               <<IH: P p_src m_src true m_tgt itr_src0 (ktr_tgt0 x)>>), *)
+  (*           P p_src m_src p_tgt m_tgt itr_src0 (ITree.bind (trigger (Choose _ X)) ktr_tgt0)) *)
+  (*       (FAILL: forall *)
+  (*           p_src m_src p_tgt m_tgt ktr_src0 itr_tgt0 *)
+  (*           id m_src0 *)
+  (*           (SRC: forall j, le (m_src0 j) (m_src j)) *)
+  (*           (FAIL: lt (m_src0 id) (m_src id)) *)
+  (*           (SIM: _isim r RR true m_src0 p_tgt m_tgt (ktr_src0 tt) itr_tgt0) *)
+  (*           (IH: P true m_src0 p_tgt m_tgt (ktr_src0 tt) itr_tgt0), *)
+  (*           P p_src m_src p_tgt m_tgt (ITree.bind (trigger (Fail id)) ktr_src0) itr_tgt0) *)
+  (*       (FAILR: forall *)
+  (*           p_src m_src p_tgt m_tgt itr_src0 ktr_tgt0 *)
+  (*           id *)
+  (*           (SIM: forall m_tgt0 (TGT: forall j, le (m_tgt0 j) (m_tgt j)) (FAIL: lt (m_tgt0 id) (m_tgt id)), *)
+  (*               (<<SIM: _isim r RR p_src m_src true m_tgt0 itr_src0 (ktr_tgt0 tt)>> /\ *)
+  (*                         (<<IH: P p_src m_src true m_tgt0 itr_src0 (ktr_tgt0 tt)>>))), *)
+  (*           P p_src m_src p_tgt m_tgt itr_src0 (ITree.bind (trigger (Fail id)) ktr_tgt0)) *)
 
-        (SUCCESSL: forall
-            p_src m_src p_tgt m_tgt ktr_src0 itr_tgt0
-            id m_src0
-            (SRC: forall j (NEQ: id <> j), le (m_src0 j) (m_src j))
-            (SIM: _isim r RR true m_src0 p_tgt m_tgt (ktr_src0 tt) itr_tgt0)
-            (IH: P true m_src0 p_tgt m_tgt (ktr_src0 tt) itr_tgt0),
-            P p_src m_src p_tgt m_tgt (ITree.bind (trigger (Success id)) ktr_src0) itr_tgt0)
-        (SUCCESSR: forall
-            p_src m_src p_tgt m_tgt itr_src0 ktr_tgt0
-            id
-            (SIM: forall m_tgt0 (TGT: forall j (NEQ: id <> j), le (m_tgt0 j) (m_tgt j)),
-                (<<SIM: _isim r RR p_src m_src true m_tgt0 itr_src0 (ktr_tgt0 tt)>>) /\
-                  (<<IH: P p_src m_src true m_tgt0 itr_src0 (ktr_tgt0 tt)>>)),
-            P p_src m_src p_tgt m_tgt itr_src0 (ITree.bind (trigger (Success id)) ktr_tgt0))
-        (PROGRESSS: forall
-            p_src m_src p_tgt m_tgt itr_src0 itr_tgt0
-            (PSRC: p_src = true)
-            (PTGT: p_tgt = true)
-            (IMAP: forall j, (<<SRC: forall n, le (m_src j) n>>) -> (<<TGT: forall n, le (m_tgt j) n>>))
-            (SIM: exists m_src0 m_tgt0, r _ _ RR false m_src0 false m_tgt0 itr_src0 itr_tgt0),
-            P p_src m_src p_tgt m_tgt itr_src0 itr_tgt0)
-    :
-    forall p_src m_src p_tgt m_tgt itr_src itr_tgt
-      (SIM: _isim r RR p_src m_src p_tgt m_tgt itr_src itr_tgt),
-      P p_src m_src p_tgt m_tgt itr_src itr_tgt.
-  Proof.
-    fix IH 7. i. inv SIM.
-    { eapply RET; eauto. }
-    { eapply TAUL; eauto. }
-    { eapply TAUR; eauto. }
-    { eapply CHOOSEL; eauto. des. esplits; eauto. }
-    { eapply CHOOSER; eauto. }
-    { eapply FAILL; eauto. }
-    { eapply FAILR; eauto. i. splits; eauto. }
-    { eapply SUCCESSL; eauto. }
-    { eapply SUCCESSR; eauto. i. split; eauto. }
-    { eapply PROGRESSS; eauto. }
-  Qed.
+  (*       (SUCCESSL: forall *)
+  (*           p_src m_src p_tgt m_tgt ktr_src0 itr_tgt0 *)
+  (*           id m_src0 *)
+  (*           (SRC: forall j (NEQ: id <> j), le (m_src0 j) (m_src j)) *)
+  (*           (SIM: _isim r RR true m_src0 p_tgt m_tgt (ktr_src0 tt) itr_tgt0) *)
+  (*           (IH: P true m_src0 p_tgt m_tgt (ktr_src0 tt) itr_tgt0), *)
+  (*           P p_src m_src p_tgt m_tgt (ITree.bind (trigger (Success id)) ktr_src0) itr_tgt0) *)
+  (*       (SUCCESSR: forall *)
+  (*           p_src m_src p_tgt m_tgt itr_src0 ktr_tgt0 *)
+  (*           id *)
+  (*           (SIM: forall m_tgt0 (TGT: forall j (NEQ: id <> j), le (m_tgt0 j) (m_tgt j)), *)
+  (*               (<<SIM: _isim r RR p_src m_src true m_tgt0 itr_src0 (ktr_tgt0 tt)>>) /\ *)
+  (*                 (<<IH: P p_src m_src true m_tgt0 itr_src0 (ktr_tgt0 tt)>>)), *)
+  (*           P p_src m_src p_tgt m_tgt itr_src0 (ITree.bind (trigger (Success id)) ktr_tgt0)) *)
+  (*       (PROGRESSS: forall *)
+  (*           p_src m_src p_tgt m_tgt itr_src0 itr_tgt0 *)
+  (*           (PSRC: p_src = true) *)
+  (*           (PTGT: p_tgt = true) *)
+  (*           (IMAP: forall j, (<<SRC: forall n, le (m_src j) n>>) -> (<<TGT: forall n, le (m_tgt j) n>>)) *)
+  (*           (SIM: exists m_src0 m_tgt0, r _ _ RR false m_src0 false m_tgt0 itr_src0 itr_tgt0), *)
+  (*           P p_src m_src p_tgt m_tgt itr_src0 itr_tgt0) *)
+  (*   : *)
+  (*   forall p_src m_src p_tgt m_tgt itr_src itr_tgt *)
+  (*     (SIM: _isim r RR p_src m_src p_tgt m_tgt itr_src itr_tgt), *)
+  (*     P p_src m_src p_tgt m_tgt itr_src itr_tgt. *)
+  (* Proof. *)
+  (*   fix IH 7. i. inv SIM. *)
+  (*   { eapply RET; eauto. } *)
+  (*   { eapply TAUL; eauto. } *)
+  (*   { eapply TAUR; eauto. } *)
+  (*   { eapply CHOOSEL; eauto. des. esplits; eauto. } *)
+  (*   { eapply CHOOSER; eauto. } *)
+  (*   { eapply FAILL; eauto. } *)
+  (*   { eapply FAILR; eauto. i. splits; eauto. } *)
+  (*   { eapply SUCCESSL; eauto. } *)
+  (*   { eapply SUCCESSR; eauto. i. split; eauto. } *)
+  (*   { eapply PROGRESSS; eauto. } *)
+  (* Qed. *)
 
-  Definition isim: forall R0 R1 (RR: R0 -> R1 -> Prop), bool -> imap  -> bool -> imap -> (itree (eventE _) R0) -> (itree (eventE _) R1) -> Prop := paco9 _isim bot9.
+  (* Definition isim: forall R0 R1 (RR: R0 -> R1 -> Prop), bool -> imap  -> bool -> imap -> (itree (eventE _) R0) -> (itree (eventE _) R1) -> Prop := paco9 _isim bot9. *)
 
-  Lemma isim_mon: monotone9 _isim.
-  Proof.
-    ii. induction IN using _isim_ind2.
-    { econs 1; eauto. }
-    { econs 2; eauto. }
-    { econs 3; eauto. }
-    { econs 4; eauto. des. esplits; eauto. }
-    { econs 5; eauto. i. hexploit SIM. i; des. eauto. }
-    { econs 6; eauto. }
-    { econs 7; eauto. i. hexploit SIM; eauto. i; des; eauto. }
-    { econs 8; eauto. }
-    { econs 9; eauto. i. hexploit SIM; eauto. i; des; eauto. }
-    { econs 10; eauto. des. esplits; eauto. }
-  Qed.
+  (* Lemma isim_mon: monotone9 _isim. *)
+  (* Proof. *)
+  (*   ii. induction IN using _isim_ind2. *)
+  (*   { econs 1; eauto. } *)
+  (*   { econs 2; eauto. } *)
+  (*   { econs 3; eauto. } *)
+  (*   { econs 4; eauto. des. esplits; eauto. } *)
+  (*   { econs 5; eauto. i. hexploit SIM. i; des. eauto. } *)
+  (*   { econs 6; eauto. } *)
+  (*   { econs 7; eauto. i. hexploit SIM; eauto. i; des; eauto. } *)
+  (*   { econs 8; eauto. } *)
+  (*   { econs 9; eauto. i. hexploit SIM; eauto. i; des; eauto. } *)
+  (*   { econs 10; eauto. des. esplits; eauto. } *)
+  (* Qed. *)
 
-  Hint Resolve isim_mon: paco.
-  Hint Resolve cpn9_wcompat: paco.
+  (* Hint Resolve isim_mon: paco. *)
+  (* Hint Resolve cpn9_wcompat: paco. *)
 
 End SIM.
 
@@ -400,11 +357,11 @@ End SIM.
 
 Section EX.
 
-  Definition Ident := nat.
+  Instance Ident : ID := mk nat.
 
   (* Definition uunit := prod unit unit. *)
 
-  Definition while_itree (step: unit -> itree (eventE Ident) (unit + unit)) : itree (eventE Ident) unit :=
+  Definition while_itree (step: unit -> itree eventE (unit + unit)) : itree eventE unit :=
     ITree.iter step tt.
 
   Lemma unfold_iter_eq A E B
@@ -447,21 +404,22 @@ Section EX.
     (* rewrite unfold_iter_eq. ired. auto. *)
 
   Definition RR := @eq nat.
+  Definition ndec := PeanoNat.Nat.eq_dec.
 
-  Definition src1 : itree (eventE Ident) nat := Ret 0.
-  Definition tgt1 : itree (eventE Ident) nat :=
-    while_itree (fun u => ITree.bind (trigger (Fail 0)) (fun r => Ret (inl r)));; Ret 0.
+  Definition src1 : itree eventE nat := Ret 0.
+  Definition tgt1 : itree eventE nat :=
+    while_itree (fun u => (trigger (Fair (fun id => (if ndec 0 id then Flag.fail else Flag.emp)))) >>= (fun r => Ret (inl r)));; Ret 0.
 
-  Goal sim RR false (@fmap_emp _) false (@fmap_emp _) 0 src1 tgt1.
+  Goal sim RR false fmap_emp false fmap_emp 0 src1 tgt1.
   Proof.
     unfold src1, tgt1.
     pcofix CIH. pfold. rewrite unfold_while_itree. ired.
     econs 7.
-    { i. instantiate (1:= fun n => if PeanoNat.Nat.eq_dec 0 n then Flag.fail else Flag.emp).
-      ss. des_ifs.
-    }
-    { i. ss. }
-    econs. econs 11; auto.
+    (* { i. instantiate (1:= fun n => if PeanoNat.Nat.eq_dec 0 n then Flag.fail else Flag.emp). *)
+    (*   ss. des_ifs. *)
+    (* } *)
+    (* { i. ss. } *)
+    econs. econs 9; auto.
     3:{ right. eauto. }
     { i. des_ifs. }
     ss.
